fix protocol bug

messageInvariantPrototypes/shardedKv/distributed/applicationProof.dfy
@@ -8,22 +8,37 @@ module ShardedKVProof {
   import opened DistributedSystem
   import opened Obligations
 
-  ghost predicate KeyInFlight(c: Constants, v: Variables, msg: Message, k: Key) 
+  ghost predicate HostsCompleteKeys(c: Constants, v: Variables)
+   requires v.WF(c)
+  {
+    forall i, k: Key | c.ValidIdx(i)
+    :: v.hosts[i].HasKey(k)
+  }
+
+
+  ghost predicate KeyInFlight(c: Constants, v: Variables, k: Key) 
+    requires v.WF(c)
+  {
+      exists msg :: KeyInFlightByMessage(c, v, msg, k)
+  }
+
+  ghost predicate KeyInFlightByMessage(c: Constants, v: Variables, msg: Message, k: Key) 
     requires v.WF(c)
   {
       && msg in v.network.sentMsgs
       && c.ValidIdx(msg.dst)
-      && msg.key.key == k
-      && (v.hosts[msg.dst].HasKey(k) ==> msg.key.version > v.hosts[msg.dst].myKeys[k])
+      && msg.key == k
+      && (v.hosts[msg.dst].HasKey(k) ==> msg.version > v.hosts[msg.dst].myKeys[k].version)
   }
 
   ghost predicate AtMostOneInFlight(c: Constants, v: Variables)
     requires v.WF(c)
   {
-    forall m1, m2, k | 
-      && KeyInFlight(c, v, m1, k) && KeyInFlight(c, v, m2, k) 
+    forall k |  KeyInFlight(c, v, k)
     ::
-      m1 == m2
+      (forall m1, m2 | 
+          KeyInFlightByMessage(c, v, m2, k) && KeyInFlightByMessage(c, v, m1, k) 
+          :: m1 == m2)
   }
 
   ghost predicate NoneHasKey(c: Constants, v: Variables, k: Key) 
@@ -36,15 +51,16 @@ module ShardedKVProof {
   ghost predicate HasKeyImpliesNoneInFlight(c: Constants, v: Variables)
     requires v.WF(c)
   {
-    forall k, msg | !NoneHasKey(c, v, k) && msg in v.network.sentMsgs
+    forall k | !NoneHasKey(c, v, k)
     ::
-    !KeyInFlight(c, v, msg, k)
+    !KeyInFlight(c, v, k)
   }
 
   
   ghost predicate ApplicationInv(c: Constants, v: Variables)
     requires v.WF(c)
   {
+    && HostsCompleteKeys (c, v)
     && AtMostOneInFlight(c, v)
     && HasKeyImpliesNoneInFlight(c, v)
   }
@@ -72,12 +88,10 @@ module ShardedKVProof {
     ensures Inv(c, v')
   {
     assert v'.WF(c);
+    InvNextHostsCompleteKeys(c, v, v');
     InvNextAtMostOneInFlight(c, v, v');
-    assert AtMostOneInFlight(c, v');
-
-    assume false;
-    assert HasKeyImpliesNoneInFlight(c, v');
-    assert Safety(c, v');
+    InvNextHasKeyImpliesNoneInFlight(c, v, v');
+    InvNextSafety(c, v, v');
   }
 
 
@@ -85,19 +99,30 @@ module ShardedKVProof {
 *                                 InvNext Proofs                                       *
 ***************************************************************************************/
 
+lemma InvNextHostsCompleteKeys(c: Constants, v: Variables, v': Variables)
+  requires v'.WF(c)
+  requires Inv(c, v)
+  requires Next(c, v, v')
+  ensures HostsCompleteKeys(c, v')
+{
+  forall i, k: Key | c.ValidIdx(i)
+  ensures v'.hosts[i].HasKey(k)
+  {
+    var dsStep :| NextStep(c, v, v', dsStep);
+    var actor, msgOps := dsStep.actor, dsStep.msgOps;
+    if actor == i {
+      assert v.hosts[i].HasKey(k);  // trigger
+    }
+  }
+}
+
 lemma InvNextAtMostOneInFlight(c: Constants, v: Variables, v': Variables)
   requires v'.WF(c)
   requires Inv(c, v)
   requires Next(c, v, v')
   ensures AtMostOneInFlight(c, v')
 {
-  forall m1, m2, k | 
-    && KeyInFlight(c, v', m1, k) && KeyInFlight(c, v', m2, k) 
-  ensures
-    m1 == m2
-  {
-    assume false;
-  }
+  assume false;
 }
 
 lemma InvNextHasKeyImpliesNoneInFlight(c: Constants, v: Variables, v': Variables)
@@ -118,39 +143,41 @@ lemma InvNextSafety(c: Constants, v: Variables, v': Variables)
   forall idx1, idx2, k: Key | 
     && c.ValidIdx(idx1) 
     && c.ValidIdx(idx2) 
-    && v'.hosts[idx1].HasKey(k)
-    && v'.hosts[idx2].HasKey(k)
+    && v'.hosts[idx1].HasLiveKey(k)
+    && v'.hosts[idx2].HasLiveKey(k)
   ensures
      idx1 == idx2
   {
     if idx1 != idx2 {
-      if v.hosts[idx1].HasKey(k) {
-        AtMostOneHostHasKey(c, v, v', k, idx1, idx2);
-      } else if v.hosts[idx2].HasKey(k) {
-        AtMostOneHostHasKey(c, v, v', k, idx2, idx1);
+      if v.hosts[idx1].HasLiveKey(k) {
+        AtMostOneHostHasLiveKey(c, v, v', k, idx1, idx2);
+      } else if v.hosts[idx2].HasLiveKey(k) {
+        AtMostOneHostHasLiveKey(c, v, v', k, idx2, idx1);
       }
     }
   }
 }
 
-lemma AtMostOneHostHasKey(c: Constants, v: Variables, v': Variables, k: Key, idx: HostId, other: HostId)
+lemma AtMostOneHostHasLiveKey(c: Constants, v: Variables, v': Variables, k: Key, idx: HostId, other: HostId)
   requires v.WF(c) && v'.WF(c)
   requires Inv(c, v)
   requires c.ValidIdx(idx)
   requires c.ValidIdx(other)
   requires idx != other
-  requires v.hosts[idx].HasKey(k)
-  requires !v.hosts[other].HasKey(k)
+  requires v.hosts[idx].HasLiveKey(k)
+  requires !v.hosts[other].HasLiveKey(k)
   requires Next(c, v, v')
-  ensures !v'.hosts[other].HasKey(k)
+  ensures !v'.hosts[other].HasLiveKey(k)
 {
   var dsStep :| NextStep(c, v, v', dsStep);
   var actor, msgOps := dsStep.actor, dsStep.msgOps;
   if actor == other {
     var cs, s, s' := c.hosts[other], v.hosts[other], v'.hosts[other];
     var step :| Host.NextStep(cs, s, s', step, msgOps);
-    if step.ReceiveStep? && v'.hosts[other].HasKey(k) {
-      assert KeyInFlight(c, v, msgOps.recv.value, k);  // trigger
+    if step.ReceiveStep? && v'.hosts[other].HasLiveKey(k) {
+      // triggers
+      assert KeyInFlightByMessage(c, v, msgOps.recv.value, k);  
+      assert KeyInFlight(c, v, k);
       assert false;
     }    
   }
