messageInvariantPrototypes/shardedKv/types.dfy
@@ -5,9 +5,9 @@ module Types {
 
   type HostId = nat
   type Key = int
-  datatype Entry = Entry(key: Key, version: nat)
+  datatype Entry = Entry(live: bool, version: nat)
 
-  datatype Message = Reconf(src: nat, dst: nat, key: Entry) 
+  datatype Message = Reconf(src: nat, dst: nat, key: Key, version: nat) 
 
   datatype MessageOps = MessageOps(recv:Option<Message>, send:Option<Message>)
 } // end module Types
